wip, a lemma about counterblocks

examples/low-level/crypto/Crypto.AEAD.Lemmas.fst
@@ -114,16 +114,41 @@ let rec extend_refines (h:mem) (i:id{safeId i}) (mac_rgn:region)
 	 cut (Seq.equal (Seq.slice ext_blocks (b + 1) (Seq.length ext_blocks)) 
 			(Seq.append blocks_tl blocks_for_e))
 
-let extending_counter_blocks (#i:id) (t:PRF.state i) (x:domain i{x.ctr <> 0ul}) 
-			     (len:u32{len <> 0ul /\ safelen i (v len) 1ul}) 
-			     (completed_len:u32{completed_len <^ len})
-			     (plain:plainBuffer i (v len)) (cipher:lbuffer (v len))
+#set-options "--z3timeout 200 --initial_fuel 2 --max_fuel 2 --initial_ifuel 0 --max_ifuel 0"
+let rec counterblocks_snoc (#i:id{safeId i}) (rgn:region) (x:domain i{x.ctr <> 0ul}) (k:nat{v x.ctr <= k})
+			 (len:nat{len <> 0 /\ safelen i len 1ul}) 
+			 (next:nat{0 < next /\ next <= v (PRF.blocklen i)})
+			 (completed_len:nat{ completed_len + next <= len /\ 
+					   FStar.Mul ((k - 1) * v (PRF.blocklen i) = completed_len)})
+			 (plain:Plain.plain i len)
+			 (cipher:lbytes len)
+   : Lemma (requires True)
+	   (ensures
+	     (let open FStar.Mul in
+	      let plain_last = Plain.slice plain completed_len (completed_len + next) in
+	      let cipher_last = Seq.slice cipher completed_len (completed_len + next) in
+	      let from = (v x.ctr - 1) * v (PRF.blocklen i) in
+	      Seq.equal (counterblocks i rgn x len from (completed_len + next) plain cipher)
+			(SeqProperties.snoc (counterblocks i rgn x len from completed_len plain cipher)
+					    (PRF.Entry ({x with ctr=UInt32.uint_to_t k}) (PRF.OTP (UInt32.uint_to_t next) plain_last cipher_last)))))
+	   (decreases (completed_len - v x.ctr))
+   = let open FStar.Mul in 
+     let from = (v x.ctr - 1) * v (PRF.blocklen i) in
+     if completed_len - from = 0
+     then ()
+     else let y = PRF.incr i x in
+          counterblocks_snoc rgn y k len next completed_len plain cipher
+
+val extending_counter_blocks: #i:id -> (t:PRF.state i) -> (x:domain i{x.ctr <> 0ul}) -> 
+			     (len:u32{len <> 0ul /\ safelen i (v len) 1ul}) -> 
+			     (completed_len:u32{completed_len <^ len}) ->
+			     (plain:plainBuffer i (v len)) -> (cipher:lbuffer (v len)) ->
 			     (h0:mem{Plain.live h0 plain /\ 
-				     Buffer.live h0 cipher})
+				     Buffer.live h0 cipher}) ->
 			     (h1:mem{Plain.live h1 plain /\ 
-				     Buffer.live h1 cipher})
-			     (h_init:mem)
-  : Lemma (requires (let remaining_len = len -^ completed_len in
+				     Buffer.live h1 cipher}) ->
+			     (h_init:mem) ->
+   Lemma (requires (let remaining_len = len -^ completed_len in
 		     let l = min remaining_len (PRF.blocklen i) in
 		     let plain_hd = Plain.sub plain completed_len l in
 		     let cipher_hd = Buffer.sub cipher completed_len l in
@@ -148,4 +173,35 @@ let extending_counter_blocks (#i:id) (t:PRF.state i) (x:domain i{x.ctr <> 0ul})
 						 (v len) 0 (v completed_len')
 						 (Plain.sel_plain h1 len plain)
 						 (Buffer.as_seq h1 cipher))))
- = admit()
+
+let extending_counter_blocks #i t x len completed_len plain cipher h0 h1 h_init
+  = if safeId i
+    then admit()
+    else ()
+
+ (*  : Lemma (requires (let remaining_len = len -^ completed_len in *)
+ (* 		     let l = min remaining_len (PRF.blocklen i) in *)
+ (* 		     let plain_hd = Plain.sub plain completed_len l in *)
+ (* 		     let cipher_hd = Buffer.sub cipher completed_len l in *)
+ (* 	             modifies_x_buffer_1 t x cipher h0 h1 /\ *)
+ (* 		    (safeId i ==>  *)
+ (* 			(HS.sel h0 t.table ==  *)
+ (* 			  Seq.append (HS.sel h_init t.table) *)
+ (* 				     (counterblocks i t.mac_rgn ({x with ctr=1ul})  *)
+ (* 						 (v len) 0 (v completed_len) *)
+ (* 						 (Plain.sel_plain h0 len plain) *)
+ (* 						 (Buffer.as_seq h0 cipher))) /\ *)
+ (* 	                ( match find_otp #t.mac_rgn #i (HS.sel h1 t.table) x with *)
+ (* 			  | Some (OTP l' p c) -> l = l' /\ p == sel_plain h1 l plain_hd /\ c == sel_bytes h1 l cipher_hd *)
+ (* 			  | None   -> False )))) *)
+ (*          (ensures (let remaining_len = len -^ completed_len in *)
+ (* 		    let l = min remaining_len (PRF.blocklen i) in *)
+ (* 		    let completed_len' = completed_len +^ l in *)
+ (* 		    safeId i ==> *)
+ (* 		      HS.sel h1 t.table == *)
+ (* 		      Seq.append (HS.sel h_init t.table)  *)
+ (* 				 (counterblocks i t.mac_rgn ({x with ctr=1ul})  *)
+ (* 						 (v len) 0 (v completed_len') *)
+ (* 						 (Plain.sel_plain h1 len plain) *)
+ (* 						 (Buffer.as_seq h1 cipher)))) *)
+ (* = admit() *)
